Lean/Geo/Triangle/TheMainTheoremNew.lean
@@ -5,19 +5,21 @@ import Geo.Triangle.EncodingNew
 namespace Geo
 open Classical LeanSAT Model
 
-axiom triangleCnfUnsat : (Geo.triangleEncoding 10 |>.toICnf compare).2.isUnsat
+axiom triangleCnfUnsat : (Geo.triangleCNF 10).isUnsat
 
-theorem EmptyTriangle10TheoremLists (pts : List Point) (gp : Point.PointListInGeneralPosition pts) (h : pts.length = 10) :
-    HasEmptyNGon 3 pts.toFinset := by
+theorem EmptyTriangle10TheoremLists (pts : List Point) (gp : Point.PointListInGeneralPosition pts)
+    (h : pts.length = 10) : HasEmptyNGon 3 pts.toFinset := by
   by_contra h'
   have noσtri : ¬σHasEmptyNGon 3 pts.toFinset := mt (σHasEmptyNGon_iff_HasEmptyNGon gp).1 h'
   have ⟨w, ⟨hw⟩⟩ := @symmetry_breaking pts (h ▸ by decide) gp
   have noσtri' : ¬σHasEmptyNGon 3 w.toFinset :=
     OrientationProperty_σHasEmptyNGon.not (hw.toEquiv w.nodup) noσtri
   have len10 : w.length = 10 := hw.length_eq.symm.trans h
-  with_reducible have := (LeanSAT.PropForm.toICnf_sat _).2 ⟨w.toPropAssn, w.satisfies_triangleEncoding noσtri'⟩
-  rw [len10] at this
-  exact triangleCnfUnsat this
+  apply triangleCnfUnsat
+  with_reducible
+    have := (LeanSAT.PropForm.toICnf_sat _).2 ⟨w.toPropAssn, w.satisfies_triangleEncoding noσtri'⟩
+    rw [len10] at this
+    rwa [triangleCNF]
 
 /- 'Geo.EmptyTriangle10TheoremLists' depends on axioms: [propext, Classical.choice, Quot.sound, Geo.cnfUnsat] -/
 #print axioms EmptyTriangle10TheoremLists
